Add crashes to the language.
Crash currently wipes block memory. It may be necessary to make it like hashmap.

src/PermProg.v
@@ -1,5 +1,5 @@
 Require Import Mem.
-Require Import AsyncDisk.
+Require Export PermAsyncDisk.
 Require Import EquivDec.
 Require Import List.
 Require Import PeanoNat.
@@ -9,78 +9,55 @@ Require Import Omega.
 Set Implicit Arguments.
 
 Definition perm := option nat. (* None can only read public blocks *)
-Definition owner := nat.
 Definition handle := nat.
-Definition block := valu.
+
 
 Definition perm_dec : forall (p p': perm), {p = p'}+{p <> p'}.
   intros; destruct p, p'; try (solve [left; auto] || solve [right; congruence]).
   destruct (Nat.eq_dec n n0); subst; auto; right; congruence.
 Defined.
 
-Inductive tag :=
-(* | Nothing : tag *)
-| Public : tag
-| Private : owner -> tag.
-
-Definition tag_dec : forall (t t': tag), {t = t'}+{t <> t'}.
-  intros; destruct t, t'; auto; try solve [right; congruence].
-  destruct (Nat.eq_dec o o0); subst; auto; right; congruence.
-Defined.
-
-Hypothesis permitted: perm -> perm -> Prop.
-
-Definition tagged_block := (tag * block)%type.
-
 Inductive op :=
 | Sea : tag -> op
-| Uns : tag -> op
-| Rn : perm -> perm -> op.
+| Uns : tag -> op.
 
 Definition op_dec : forall (o o': op), {o = o'}+{o <> o'}.
   intros.
   destruct o, o'; auto; try (solve [right; congruence] ||
   solve [destruct (tag_dec t t0); subst; auto; right; congruence]).
-  destruct (perm_dec p p1); subst; try solve [right; congruence].
-  destruct (perm_dec p0 p2); subst; auto; right; congruence.
 Defined.
 
 Definition trace := list op.
-Definition tagged_disk:= @Mem.mem addr addr_eq_dec tagged_block.
-Definition block_mem:= @Mem.mem handle Nat.eq_dec tagged_block.
+Definition handle_eq_dec:= Nat.eq_dec.
+Definition tagged_disk:= rawdisk.
+Definition block_mem:= @Mem.mem handle handle_eq_dec tagged_block.
 
 Inductive result : Type :=
-| Finished : forall T, tagged_disk -> block_mem -> T -> result.
-
+| Finished : forall T, tagged_disk -> block_mem -> T -> result
+| Crashed : tagged_disk -> result.
 
 Inductive prog : Type -> Type :=
 | Read : addr -> prog handle
 | Write : addr -> handle -> prog unit
 | Seal : tag -> block -> prog handle
 | Unseal : handle -> prog block
-(* 
-| GetTag : handle -> prog tag
-| Clear : handle -> prog unit (* Clears the blocks memory. May simplify security specs *)
-| Purge : addr -> prog unit (* Clears a block and sets its tag to 'Nothing' *) 
-*)
 | Ret : forall T, T -> prog T
-| Run : forall T, perm -> prog T -> prog T
 | Bind: forall T T', prog T  -> (T -> prog T') -> prog T'.
 
 Notation "x <- p1 ;; p2" := (Bind p1 (fun x => p2))
                               (at level 60, right associativity).
 
-Inductive  exec:
+Inductive exec:
   forall T, perm -> trace -> tagged_disk ->
        block_mem -> prog T ->  result -> trace -> Prop :=
-| ExecRead    : forall pr d bm a i tb tr,
+| ExecRead    : forall pr d bm a i tb tbs tr,
                   bm i = None ->
-                  d a = Some tb ->
+                  d a = Some (tb, tbs) ->
                   exec pr tr d bm (Read a) (Finished d (upd bm i tb) i) tr                 
-| ExecWrite   : forall pr d bm a i tb tr,
+| ExecWrite   : forall pr d bm a i tb tbs tr,
                   bm i = Some tb ->
-                  d a <> None ->
-                  exec pr tr d bm (Write a i) (Finished (upd d a tb) bm tt) tr
+                  d a = Some tbs ->
+                  exec pr tr d bm (Write a i) (Finished (upd d a (tb, vsmerge tbs)) bm tt) tr
                        
 | ExecSeal : forall pr d bm i t b tr,
                bm i = None ->
@@ -89,27 +66,31 @@ Inductive  exec:
 | ExecUnseal : forall pr d bm i tb tr,
                  bm i = Some tb ->
                  exec pr tr d bm (Unseal i) (Finished d bm (snd tb)) (Uns (fst tb)::tr)
-(* 
-| ExecGetTag : forall o s i t b tr,
-                 blocks s i = Some (t, b) ->
-                 t <> Nothing ->
-                 exec o s tr (GetTag i) s (Finished t) tr
-                      
-| ExecClear : forall o h s tr,
-                exec o s tr (Clear h)  (mkstate (disk s)
-                                                (mem_except Nat.eq_dec (blocks s) h)) (Finished tt) tr
-| ExecPurge :  forall o a s tr,
-                 exec o s tr (Purge a)  (disk_upd s a (Nothing, 0)) (Finished tt) tr
-*)                      
+
 | ExecRet : forall T pr d bm (r: T) tr,
               exec pr tr d bm (Ret r) (Finished d bm r) tr
-                   
-| ExecRun : forall T pr pr' d bm r (p: prog T) tr tr',
-              exec pr' tr d bm p r tr' ->
-              exec pr tr d bm (Run pr' p) r (Rn pr pr'::tr')
                    
 | ExecBind : forall T T' pr (p1 : prog T) (p2: T -> prog T') d bm d' bm' v r tr tr' tr'',
                exec pr tr d bm p1 (Finished d' bm' v) tr' ->
                exec pr tr' d' bm' (p2 v) r tr'' ->
-               exec pr tr d bm (Bind p1 p2) r tr''.
+               exec pr tr d bm (Bind p1 p2) r tr''
+                      
+| CrashRead : forall pr d bm a tr,
+                exec pr tr d bm (Read a) (Crashed d) tr
+                        
+| CrashWrite : forall pr d bm a i tr,
+                 exec pr tr d bm (Write a i) (Crashed d) tr
+                         
+| CrashSeal : forall pr d bm t b tr,
+                exec pr tr d bm (Seal t b) (Crashed d) tr
+                        
+| CrashUnseal : forall pr d bm i tr,
+                exec pr tr d bm (Unseal i) (Crashed d) tr
+                    
+| CrashRet : forall T pr d bm (r: T) tr,
+              exec pr tr d bm (Ret r) (Crashed d) tr
 
+| CrashBind : forall T T' pr (p1 : prog T) (p2: T -> prog T') d d' bm tr tr' r,
+                exec pr tr d bm p1 r tr' ->
+                r = (Crashed d') ->
+                exec pr tr d bm (Bind p1 p2) r tr'.
