src/PermProgMonad.v
@@ -1,69 +1,7 @@
-Require Import PermProg PermProgAuto.
-Require Import PermSec PermHoare.
+Require Export PermSec.
 Require Import ProofIrrelevance.
 
 Set Implicit Arguments.
-
-(*Ltac inj_existT :=
-  match goal with
-  | [ H: existT ?P ?p _ = existT ?P ?p _ |- _ ] =>
-    apply inj_pair2 in H
-  end.
-
-Ltac inv_step :=
-  match goal with
-  | [ H: step _ _ _ _ _ _ _ _ |- _ ] =>
-    inversion H;
-    repeat inj_existT;
-    subst;
-    clear H
-  end.
-
-Ltac inv_fail_step :=
-  try match goal with
-      | [ H: exec _ _ _ _ (Failed _) |- _ ] =>
-        inversion H; repeat inj_existT; subst; clear H
-      end;
-  match goal with
-  | [ H: fail_step _ _ _ |- _ ] =>
-    inversion H; subst; clear H
-  end.
-
-Ltac inv_crash_step :=
-  try match goal with
-      | [ H: exec _ _ _ _ (Crashed _ _ _) |- _ ] =>
-        inversion H; repeat inj_existT; subst; clear H
-      end;
-  match goal with
-  | [ H: crash_step _ |- _ ] =>
-    inversion H; subst; clear H
-  end.
-
-Ltac inv_exec' H :=
-    inversion H;
-    repeat inj_existT; subst;
-    try inv_step;
-    try inv_fail_step;
-    try inv_crash_step;
-    subst;
-    clear H.
-
-Ltac inv_exec :=
-  lazymatch goal with
-  | [ H: exec _ _ _ (Ret _) _ |- _ ] =>
-    inv_exec' H
-  | [ H: exec _ _ _ (AlertModified) _ |- _ ] =>
-    inv_exec' H
-  | [ H: exec _ _ _ (Debug _ _) _ |- _ ] =>
-    inv_exec' H
-  | [ H: exec _ _ _ (Bind _ _) _ |- _ ] =>
-    inv_exec' H
-  | [ H: exec _ _ _ _ _ |- _ ] =>
-    inv_exec' H
-  end.
- *)
-
-Section MonadLaws.
 
   Definition prog_equiv T : prog T -> prog T -> Prop :=
     fun p1 p2 => forall pr tr d bm tr' out,
@@ -73,23 +11,46 @@ Section MonadLaws.
 
   Infix "~=" := prog_equiv (at level 50, left associativity).
 
-  Theorem bind_left_id : forall T T' v (p: T -> prog T'),
-      Bind (Ret v) p ~= p v.
-  Proof.
-    split; intros.
-    - inv_exec_perm.
-      inv_exec_perm; eauto.
-    - repeat econstructor; eauto.
-  Qed.
-
   Theorem bind_assoc : forall T T' T'' (p1: prog T) (p2: T -> prog T') (p3: T' -> prog T''),
       Bind (Bind p1 p2) p3 ~= Bind p1 (fun x => Bind (p2 x) p3).
   Proof.
     split; intros.
-    - repeat inv_exec_perm; eauto;
+    inv_exec_perm.
+    {
+      destruct out; cleanup.
+      {
+        inv_exec_perm.
+        repeat econstructor; eauto.
+      }
+      split_ors.
+      {
+        inv_exec_perm; cleanup.
+        split_ors; cleanup.
+        eapply CrashBind; auto.
+
+        econstructor; eauto.
+        eapply CrashBind; eauto.
+      }
+
+      {
+        inv_exec_perm.
+        repeat econstructor; eauto.
+      }
+    }
+
+    inv_exec_perm.
+    {
+      destruct out; cleanup.
+      inv_exec_perm.
       repeat econstructor; eauto.
-    - repeat inv_exec_perm; eauto.
+      split_ors.
+      repeat eapply CrashBind; eauto.
+      inv_exec_perm.
+      split_ors.
+      eapply CrashBind;
+      econstructor; eauto.
       repeat econstructor; eauto.
+    }
   Qed.
 
   Theorem security_equivalence:
@@ -104,30 +65,3 @@ Section MonadLaws.
       edestruct H; eauto
     end.
   Qed.
-  
-  Theorem corr2_equivalence :
-    forall T pr (p p': prog T) pre,
-      corr2 pr pre p' ->
-      prog_equiv p p' ->
-      corr2 pr pre p.
-  Proof.
-    unfold corr2; intros.
-    match goal with
-    | [ H: _ ~= _ |- _ ] =>
-      edestruct H; eauto
-    end.
-    edestruct H; eauto.
-    intuition.
-    eapply security_equivalence; eauto.
-  Qed.
-
-End MonadLaws.
-Print corr2.
-Ltac monad_simpl_one :=
-  match goal with
-  | [ |- corr2 _ _ (Bind (Bind _ _) _) ] =>
-    eapply corr2_equivalence;
-    [ | apply bind_assoc ]
-  end.
-
-Ltac monad_simpl := repeat monad_simpl_one.
